Update matchingBlood.dfy

matchingBlood.dfy
@@ -5,44 +5,65 @@ import B = BloodRep
 datatype BloodType = A | B | AB | O // A = 0, B = 1, AB = 2, O = 3
 datatype BloodRecord = BloodRecord(bType: BloodType, location: string, donationDate: D.Date, expiryDate: D.Date, isOkay: bool)
 
-method matchingBlood(patientBloodType: BloodType, a:array<BloodRecord>) returns (compatibleBlood: bool)
+
+method GetCompatibleBlood(patientBloodType: BloodType, a:array<BloodRecord>) returns (compatibleBlood: BloodRecord)
+    requires a != null && a.Length > 0
+    requires compatibleBloodExists(patientBloodType, a)
+    ensures isCompatible(patientBloodType, compatibleBlood.bType)
+{
+    var i := 0;
+    while (i < a.Length)
+        decreases a.Length - i
+        invariant 0 <= i <= a.Length
+        invariant forall k :: 0 <= k < i ==> !isCompatible(patientBloodType, a[k].bType)
+    {
+        var comp := AreCompatible(patientBloodType, a[i].bType);
+        if (comp)
+        {
+            compatibleBlood := a[i];
+        }
+        i := i + 1;
+    }
+}
+
+method CompatibleBloodExists(patientBloodType: BloodType, a:array<BloodRecord>) returns (compatibleBlood: bool)
     requires a != null && a.Length > 0
     ensures compatibleBlood == compatibleBloodExists(patientBloodType, a)
 {
     // Check Type O Compatibility
     if (patientBloodType == O)
     {
-        compatibleBlood := doesExist(O, a);
+        compatibleBlood := DoesExist(O, a);
     }
 
     // Check Type A Compatibility
     else if (patientBloodType == A)
     {
-        var existsA := doesExist(A, a);
-        var existsO := doesExist(O, a);
+        var existsA := DoesExist(A, a);
+        var existsO := DoesExist(O, a);
         compatibleBlood := (existsA || existsO);
     }
 
     // Check type B Compatibility
     else if (patientBloodType == B)
     {
-        var existsB := doesExist(B, a);
-        var existsO := doesExist(O, a);
+        var existsB := DoesExist(B, a);
+        var existsO := DoesExist(O, a);
         compatibleBlood := (existsB || existsO);
     }
 
     // Check AB Compatibility
     else if (patientBloodType == AB)
     {
-        var existsA := doesExist(A, a);
-        var existsB := doesExist(B, a);
-        var existsAB := doesExist(AB, a);
-        var existsO := doesExist(O, a);
+        var existsA := DoesExist(A, a);
+        var existsB := DoesExist(B, a);
+        var existsAB := DoesExist(AB, a);
+        var existsO := DoesExist(O, a);
         compatibleBlood := (existsA || existsB || existsAB || existsO);
     }
 }
 
-method doesExist(bType: BloodType, a:array<BloodRecord>) returns (Exists: bool)
+method DoesExist(bType: BloodType, a:array<BloodRecord>) returns (Exists: bool)
     requires a != null
     ensures Exists == exists k :: 0 <= k < a.Length && a[k].bType == bType
 {
@@ -62,11 +83,14 @@ method doesExist(bType: BloodType, a:array<BloodRecord>) returns (Exists: bool)
     }
 }
 
-// predicate doesExistPredicate(bType: BloodType, a:array<BloodRecord>)
-//     reads a
-// {
-//     exists k :: 0 <= k < a.Length && a[k].bType == bType
-// }
+method AreCompatible(patientBloodType: BloodType, donorBloodType: BloodType) returns (areCompatible: bool)
+    ensures isCompatible(patientBloodType, donorBloodType)
+{
+    areCompatible := (patientBloodType == O && donorBloodType == O) ||
+        (patientBloodType == A && (donorBloodType == O || donorBloodType == A)) ||
+        (patientBloodType == B && (donorBloodType == O || donorBloodType == B)) ||
+        (patientBloodType == AB && (donorBloodType == O || donorBloodType == A || donorBloodType == B || donorBloodType == AB));
+}
 
 predicate compatibleBloodExists(bType: BloodType, a:array<BloodRecord>)
     reads a
@@ -78,3 +102,14 @@ predicate compatibleBloodExists(bType: BloodType, a:array<BloodRecord>)
         case AB => exists i :: 0 <= i < a.Length && (a[i].bType == O || a[i].bType == A || a[i].bType == B || a[i].bType == AB)
     }
 }
+
+predicate isCompatible(bType1: BloodType, bType2: BloodType)
+{ match(bType1)
+    {
+        case O => bType2 == O
+        case A => bType2 == O || bType2 == A
+        case B => bType2 == O || bType2 == B
+        case AB => bType2 == O || bType2 == AB
+    }
+}
+
